Dafny/Printer.cs
@@ -574,7 +574,9 @@ namespace Microsoft.Dafny {
       } else if (stmt is ParallelStmt) {
         var s = (ParallelStmt)stmt;
         wr.Write("parallel (");
-        PrintQuantifierDomain(s.BoundVars, s.Attributes, s.Range);
+        if (s.BoundVars.Count != 0) {
+          PrintQuantifierDomain(s.BoundVars, s.Attributes, s.Range);
+        }
         if (s.Ens.Count == 0) {
           wr.Write(") ");
         } else {
